- some corrected names and evaluating an operator in a computable input.

baire_spaces/countability/seq_cont.v
@@ -48,17 +48,38 @@ Section sequential_continuity.
     exact/scnt_frcs.
   Qed.
 
-  Lemma cont_scnt: F \is_continuous -> sequentially_continuous.
+  Definition continuity_point phi :=
+    forall Fphi, F phi Fphi -> exists Lf, Lf \is_modulus_of F \on_input phi.
+
+  Lemma cntp_spec: F \is_continuous <-> forall phi, continuity_point phi.
   Proof.
-    move => cont phi phin Fphin Fphi lim vals val L.
-    have [Lf mod]:= cont phi Fphi val.
+    split => [cont phi Fphi val | cont].
+    - by have [Lf]:= cont phi Fphi val; exists Lf => q'; exists (Fphi q').
+    apply/cont_spec => phi [Fphi val].
+    exact/cont/val.
+  Qed.
+
+  Lemma imod_spec Lf phi Fphi: F phi Fphi -> Lf \is_modulus_of F \on_input phi <->
+    forall q', certificate F (Lf q') phi q' (Fphi q').
+  Proof.
+    move => val; split => mod q'; last by exists (Fphi q').
+    by have [a' crt]:= mod q'; apply/crt_icf/crt/val.
+  Qed.
+    
+  Lemma cntp_scntp phi: continuity_point phi -> sequential_continuity_point phi.
+  Proof.
+    move => cont phin Fphin Fphi lim vals val L.
+    have [Lf /(imod_spec _ val) mod]:= cont Fphi val.
     have [n prp]:= lim (gather Lf L).
     exists n => m ineq.
     elim: L prp => [ | q' L ih prp]//.
     split; last by apply/ih => m' ineq'; have /coin_cat []:= prp m' ineq'.
     symmetry; apply/mod/vals.
-    by have /coin_cat []:= prp m ineq.
+    by have /coin_cat []:= prp m ineq.    
   Qed.
+
+  Lemma cont_scnt: F \is_continuous -> sequentially_continuous.
+  Proof. by move => /cntp_spec cont phi; apply/cntp_scntp/cont. Qed.
 End sequential_continuity.
 Notation "F \is_sequentially_continuous_in phi" := (sequential_continuity_point F phi) (at level 40): baire_scope.
 Notation "F \is_sequentially_continuous" := (sequentially_continuous F) (at level 40): baire_scope.
